theories/modules/SModTr.v
@@ -98,7 +98,7 @@ Section HOARE.
     λ '(sp,fsp) bd, HoareFun fsp (trans sp ∘ bd).
 
   Definition trans_ktree sp (sb: fnsem_type (option fspec * fbody)) : fnsem_type fbody :=
-    map_snd (λ '(fsp,bd), trans_body (if sb.1.1.1 then (sp, fsp) else (sp_none, None)) bd) sb.
+    map_snd (λ '(fsp,bd), trans_body (if sb.1.1.1 then sp else sp_none, fsp) bd) sb.
 
 End HOARE.
 End SModTr.
